typing.v
@@ -1,0 +1,150 @@
+From iris.program_logic Require Import thread_local hoare.
+From lrust Require Export type perm notation.
+From lrust Require Import type_incl perm_incl proofmode.
+
+Import Types Perm.
+
+Section typing.
+
+  Context `{heapG Σ, lifetimeG Σ, thread_localG Σ}.
+
+  (* TODO : good notations for [typed_step] and [typed_step_ty] ? *)
+  Definition typed_step (ρ : perm) e (θ : Valuable.t → perm) :=
+    ∀ tid, {{ ρ tid ★ tl_own tid ⊤ }} e {{ v, θ (Some v) tid ★ tl_own tid ⊤ }}.
+
+  (* FIXME : why isn't the notation context on the last parameter not
+     taken into account? *)
+  Arguments typed_step _%P _%E _%P.
+
+  Definition typed_step_ty (ρ : perm) e ty :=
+    typed_step ρ e (λ ν, ν ◁ ty)%P.
+
+  Definition typed_program (ρ : perm) e :=
+    ∀ tid, {{ ρ tid ★ tl_own tid ⊤ }} e {{ v, False }}.
+
+  Lemma typed_step_frame ρ e θ ξ:
+    typed_step ρ e θ → typed_step (ρ ★ ξ) e (λ ν, θ ν ★ ξ)%P.
+  Proof. iIntros (Hwt tid) "!#[[?$]?]". iApply Hwt. by iFrame. Qed.
+
+  Lemma typed_step_exists {A} ρ θ e ξ:
+    (∀ x:A, typed_step (ρ ★ θ x) e ξ) →
+    typed_step (ρ ★ ∃ x, θ x) e ξ.
+  Proof.
+    iIntros (Hwt tid) "!#[[Hρ Hθ]?]". iDestruct "Hθ" as (x) "Hθ".
+    iApply Hwt. by iFrame.
+  Qed.
+
+  Lemma typed_step_bool ρ (b:Datatypes.bool) :
+    typed_step_ty ρ #b bool.
+  Proof. iIntros (tid) "!#[_$]". wp_value. simpl. eauto. Qed.
+
+  Lemma typed_step_int ρ (z:Datatypes.nat) :
+    typed_step_ty ρ #z int.
+  Proof. iIntros (tid) "!#[_$]". wp_value. simpl. eauto. Qed.
+
+  Lemma typed_step_fn {A n} `{Duplicable _ ρ, Closed (f :b: xl +b+ []) e} θ :
+    length xl = n →
+    (∀ (a : A) (vl : vec val n) (fv : val) e',
+        subst_l xl (map of_val vl) e = Some e' →
+        typed_program (Some fv ◁ fn θ ★ (θ a vl) ★ ρ) (subst' f fv e')) →
+    typed_step_ty ρ (Rec f xl e) (fn θ).
+  Proof.
+    iIntros (Hn He tid) "!# [#Hρ $]". iApply (wp_value _ _ _ (RecV f xl e)).
+    { simpl. destruct decide as [CL|?]. repeat f_equal. apply proof_irrel. done. }
+    iLöb as "IH". iExists _. iSplit. done. iIntros (a vl) "!#[Hθ?]".
+    assert (is_Some (subst_l xl (map of_val vl) e)) as [e' He'].
+    { clear -Hn. revert xl Hn e. induction vl=>-[|x xl] //=. by eauto.
+      intros ? e. edestruct IHvl as [e' ->]. congruence. eauto. }
+    iApply wp_rec; try done.
+    { apply List.Forall_forall=>?. rewrite in_map_iff=>-[?[<- _]].
+      rewrite to_of_val. eauto. }
+    iNext. iApply He. done. by iFrame "★#".
+  Qed.
+
+  Lemma typed_step_cont {n} `{Closed (f :b: xl +b+ []) e} ρ θ :
+    length xl = n →
+    (∀ (vl : vec val n) (fv : val) e',
+        subst_l xl (map of_val vl) e = Some e' →
+        typed_program (Some fv ◁ cont (λ vl, ρ ★ θ vl)%P ★ (θ vl) ★ ρ) (subst' f fv e')) →
+    typed_step_ty ρ (Rec f xl e) (cont θ).
+  Proof.
+    iIntros (Hn He tid) "!# [Hρ $]". iApply (wp_value _ _ _ (RecV f xl e)).
+    { simpl. destruct decide as [CL|?]. repeat f_equal. apply proof_irrel. done. }
+    iLöb as "IH". iExists _. iSplit. done. iIntros (vl) "Hθ ?".
+    assert (is_Some (subst_l xl (map of_val vl) e)) as [e' He'].
+    { clear -Hn. revert xl Hn e. induction vl=>-[|x xl] //=. by eauto.
+      intros ? e. edestruct IHvl as [e' ->]. congruence. eauto. }
+    iApply wp_rec; try done.
+    { apply List.Forall_forall=>?. rewrite in_map_iff=>-[?[<- _]].
+      rewrite to_of_val. eauto. }
+    iNext. iApply He. done. iFrame. simpl.
+    iExists _. iSplit. done. iIntros (vl') "[Hρ Hθ] Htl".
+    iDestruct ("IH" with "Hρ") as (f') "[Hf' IH']".
+    iDestruct "Hf'" as %[=<-]. iApply ("IH'" with "Hθ Htl").
+  Qed.
+
+  Lemma typed_step_valuable e ty:
+    typed_step_ty (Valuable.of_expr e ◁ ty) e ty.
+  Proof.
+    iIntros (tid) "!#[H$]".
+    destruct (Valuable.of_expr e) as [v|] eqn:Hv. 2:by iDestruct "H" as "[]".
+    by iApply Valuable.of_expr_wp.
+  Qed.
+
+  Lemma typed_step_plus e1 e2 ρ1 ρ2:
+    typed_step_ty ρ1 e1 int → typed_step_ty ρ2 e2 int →
+    typed_step_ty (ρ1 ★ ρ2) (BinOp PlusOp e1 e2) int.
+  Proof.
+    iIntros (He1 He2 tid) "!#[[H1 H2]?]".
+    wp_bind e1. iApply wp_wand_r. iSplitR "H2". iApply He1; by iFrame.
+    iIntros (v1) "[Hv1?]". iDestruct "Hv1" as (z1) "Hz1". iDestruct "Hz1" as %[=->].
+    wp_bind e2. iApply wp_wand_r. iSplitL. iApply He2; by iFrame.
+    iIntros (v2) "[Hv2?]". iDestruct "Hv2" as (z2) "Hz2". iDestruct "Hz2" as %[=->].
+    wp_op. iFrame. by iExists _.
+  Qed.
+
+  Lemma typed_step_minus e1 e2 ρ1 ρ2:
+    typed_step_ty ρ1 e1 int → typed_step_ty ρ2 e2 int →
+    typed_step_ty (ρ1 ★ ρ2) (BinOp MinusOp e1 e2) int.
+  Proof.
+    iIntros (He1 He2 tid) "!#[[H1 H2]?]".
+    wp_bind e1. iApply wp_wand_r. iSplitR "H2". iApply He1; by iFrame.
+    iIntros (v1) "[Hv1?]". iDestruct "Hv1" as (z1) "Hz1". iDestruct "Hz1" as %[=->].
+    wp_bind e2. iApply wp_wand_r. iSplitL. iApply He2; by iFrame.
+    iIntros (v2) "[Hv2?]". iDestruct "Hv2" as (z2) "Hz2". iDestruct "Hz2" as %[=->].
+    wp_op. iFrame. by iExists _.
+  Qed.
+
+  Lemma typed_step_le e1 e2 ρ1 ρ2:
+    typed_step_ty ρ1 e1 int → typed_step_ty ρ2 e2 int →
+    typed_step_ty (ρ1 ★ ρ2) (BinOp LeOp e1 e2) bool.
+  Proof.
+    iIntros (He1 He2 tid) "!#[[H1 H2]?]".
+    wp_bind e1. iApply wp_wand_r. iSplitR "H2". iApply He1; by iFrame.
+    iIntros (v1) "[Hv1?]". iDestruct "Hv1" as (z1) "Hz1". iDestruct "Hz1" as %[=->].
+    wp_bind e2. iApply wp_wand_r. iSplitL. iApply He2; by iFrame.
+    iIntros (v2) "[Hv2?]". iDestruct "Hv2" as (z2) "Hz2". iDestruct "Hz2" as %[=->].
+    iFrame. wp_op; intros _; by iExists _.
+  Qed.
+
+  Lemma typed_step_newlft ρ:
+    typed_step ρ Newlft (λ _, ∃ α, [α]{1} ★ α ∋ top)%P.
+  Proof.
+    iIntros (tid) "!#[_$]". wp_value. iVs lft_begin as (α) "[?#?]". done.
+    iVs (lft_borrow_create with "[][]") as "[_?]". done. done.
+    2:by iVsIntro; iExists α; iFrame. eauto.
+  Qed.
+
+  Lemma typed_step_endlft κ ρ:
+    typed_step (κ ∋ ρ ★ [κ]{1}) Endlft (λ _, ρ)%P.
+  Proof.
+    iIntros (tid) "!#[[Hextr [Htok #Hlft]]$]".
+    wp_bind (#() ;; #())%E.
+    iApply (wp_wand_r _ _ (λ _, _ ★ True)%I). iSplitR "Hextr".
+    iApply (wp_frame_step_l with "[-]"); try done.
+    iDestruct (lft_end with "Hlft Htok") as "$". by wp_seq.
+    iIntros (v) "[#Hκ _]". iVs (lft_extract_out with "Hκ Hextr"). done.
+    by wp_seq.
+  Qed.
+
+End typing.
